more work on the modular iterator functions specs

verif/db/verif_operations.v
@@ -2,14 +2,17 @@ Require Import VST.floyd.proofauto.
 Require Import VST.floyd.library.
 Require Import VST.msl.iter_sepcon.
 Require Signatures.
-Require btrees.btrees.
-Require btrees.btrees_sep. Require btrees.btrees_spec.
 Require FiniteSet FlatData SortedTuples SortedAttributes Values Plans.
 Require SeqScan.
 Require db_operations.
+Require VST.progs.verif_queue2.
+Require relation_mem.
+
+Require Program.Basics. Require Program.Combinators.
 
 Section Tuple.
   Import Values SortedAttributes FiniteSet FlatData Plans.
+  Import Program.Basics Program.Combinators.
   Fixpoint string_to_list_byte (s: string) : list byte :=
     match s with
     | EmptyString => nil
@@ -27,11 +30,24 @@ Section Tuple.
   (* This need to be implemented. *)
   Definition stringpool_rep (sp : stringpool) : mpred := emp.
 
-  Definition tuple := Tuple.tuple TPL.T.
-  Definition support : tuple -> setA := Tuple.support TPL.T.
+  Definition tuple : Type := Tuple.tuple TPL.T * val. (* Augmented type *)
+  Definition support : tuple -> setA := Tuple.support TPL.T ∘ fst.
   Definition attribute := Tuple.attribute TPL.T.
-  Definition dot : tuple -> attribute -> value := Tuple.dot TPL.T. Check dot.
-  Definition Otuple : OrderedSet.Oeset.Rcd tuple := Tuple.OTuple TPL.T.
+  Definition dot : tuple -> attribute -> value := Tuple.dot TPL.T ∘ fst.
+  Section Otuple.
+    Import OrderedSet.Oeset.
+    Definition Otuple' : OrderedSet.Oeset.Rcd (FlatData.Tuple.tuple TPL.T) := Tuple.OTuple TPL.T.
+    Program Definition Otuple : OrderedSet.Oeset.Rcd tuple :=
+      {|
+        compare := fun '(t1, p1) '(t2, p2) => Otuple'.(compare) t1 t2 ;
+        compare_eq_trans := fun '(t1, p1) '(t2, p2) '(t3, p3) h12 h23 => Otuple'.(compare_eq_trans) t1 t2 t3 h12 h23 ;
+        compare_eq_lt_trans :=  fun '(t1, p1) '(t2, p2) '(t3, p3) h12 h23 => Otuple'.(compare_eq_lt_trans) t1 t2 t3 h12 h23 ;
+        compare_lt_eq_trans :=  fun '(t1, p1) '(t2, p2) '(t3, p3) h12 h23 => Otuple'.(compare_lt_eq_trans) t1 t2 t3 h12 h23 ;
+        compare_lt_trans :=  fun '(t1, p1) '(t2, p2) '(t3, p3) h12 h23 => Otuple'.(compare_lt_trans) t1 t2 t3 h12 h23 ;
+        compare_lt_gt := fun '(t1, p1) '(t2, p2) => Otuple'.(compare_lt_gt) t1 t2
+      |}.
+  End Otuple.
+
   Global Opaque tuple support attribute dot Otuple.
 
   Definition tuple_rep (sh : share) (t : tuple) (p : val) : mpred :=
@@ -40,20 +56,11 @@ Section Tuple.
                     (map (val_of_value sp oo dot t) ({{{support t}}})) p * stringpool_rep sp.
 End Tuple. 
 
-Section CompSpecs.
-  
-  Definition db_operations_CompSpecs : compspecs. make_compspecs db_operations.prog. Defined.
-  Definition db_operations_Vprog : varspecs. mk_varspecs db_operations.prog. Defined.
-
-  Definition relation_mem_CompSpecs : compspecs. make_compspecs relation_mem.prog. Defined.
-  Definition relation_mem_Vprog : varspecs. mk_varspecs relation_mem.prog. Defined.
-  
-End CompSpecs.
+Instance CompSpecs : compspecs. make_compspecs db_operations.prog. Defined.
+Definition Vprog : varspecs. mk_varspecs db_operations.prog. Defined.
 
 Section AttrList.
   Import db_operations SortedAttributes FiniteSet.
-
-  Existing Instance db_operations_CompSpecs.
   
   Definition t_attr_list_t := Tstruct _attribute_list_t noattr.
   
@@ -131,392 +138,144 @@ Section AttrList.
   Definition attribute_list_length_spec :=
     DECLARE _attribute_list_length
             WITH sh: share, l: val, attrs: Fset.set FAN
-                                                    PRE [ _l OF (tptr t_attr_list_t)]
-                                                    PROP(readable_share sh)
-                                                    LOCAL (temp _l l; temp _x l)
-                                                    SEP (attributes_rep sh attrs l)
-                                                    POST [ size_t ]
-                                                    PROP()
-                                                    LOCAL(temp ret_temp (Vint (Int.repr (Z.of_nat (Fset.cardinal _ attrs)))))
-                                                    SEP (attributes_rep sh attrs l).
-
+                PRE [ _l OF (tptr t_attr_list_t)]
+                PROP(readable_share sh)
+                LOCAL (temp _l l; temp _x l)
+                SEP (attributes_rep sh attrs l)
+                POST [ size_t ]
+                PROP()
+                LOCAL(temp ret_temp (Vint (Int.repr (Z.of_nat (Fset.cardinal _ attrs)))))
+                SEP (attributes_rep sh attrs l).
 
 End AttrList.
 
 Section Iterator.
   Import db_operations FlatData Plans Signatures.
   
-  Existing Instance db_operations_CompSpecs.
-  
   Definition t_iterator_t := Tstruct _iterator_t noattr.
   Definition t_methods := Tstruct _methods noattr.
   Definition t_seq_scan_env := Tstruct _seq_scan_env noattr.
   Definition t_index_join_env := Tstruct _index_join_env noattr.
-
-  Record iterator_class (c: Cursor.Rcd Otuple) :=
-    {
-      env: Type;
-      env_assert: env -> Cursor.cursor c -> val -> mpred;
-      env_init: env -> env;
-      env_next: env -> env;
-      (* +axioms *)
-      env_close: env -> env;
-    }.
-  Arguments env {c}.
-  Arguments env_assert {c}.
-  Arguments env_init {c}.
-  Arguments env_next {c}.
-  Arguments env_close {c}.
-
+  Definition t_fifo := Tstruct _fifo noattr.
+  Import QEP.
+  Definition iterator_invariant (c: cursor): Type := Cursor.cursor (type_cursor c) -> val -> mpred.
+    
   Definition result_rep sh (r : result tuple) (p: val) : mpred :=
     match r with
     | Result t => tuple_rep sh t p
     | No_Result => emp (* ??? *)
     | Empty_Cursor => !! (p = nullval) end.
-
-  Definition next_spec {c: Cursor.Rcd Otuple} (cl : iterator_class c) :=
-    WITH p: val, e: env cl, it: Cursor.cursor c, sh: share, gv: globals
+  
+  Definition init_spec {c: cursor} (instance: iterator_invariant c) :=
+    WITH sh: share, gv: globals, penv: val, c: Cursor.cursor (type_cursor c)
   PRE [ _env OF (tptr tvoid) ]
-  PROP(Cursor.coherent it)
-  LOCAL(gvars gv; temp _env p)
-  SEP(mem_mgr gv; env_assert cl e it p)
+    PROP(Cursor.coherent c)
+    LOCAL(gvars gv; temp _env penv)
+    SEP(mem_mgr gv; instance c penv)
+  POST [ tvoid ]
+    PROP()
+    LOCAL()
+    SEP(mem_mgr gv; instance (Cursor.reset c) penv).
+
+  Definition next_spec {c: cursor} (instance: iterator_invariant c) :=
+    WITH sh: share, gv: globals, penv: val, c: Cursor.cursor (type_cursor c)
+  PRE [ _env OF (tptr tvoid) ]
+    PROP(Cursor.coherent c)
+    LOCAL(gvars gv; temp _env penv)
+    SEP(mem_mgr gv; instance c penv)
   POST [ tptr tvoid ]
-  EX t: val,
-  PROP()
-  LOCAL(temp ret_temp t)
-  SEP(mem_mgr gv; result_rep sh (fst (Cursor.next it)) t; cl.(env_assert) (cl.(env_next) e) (snd (Cursor.next it)) p).
+  let '(res, next_c) := Cursor.next c in
+  EX pres: val,
+    PROP()
+    LOCAL(temp ret_temp pres)
+    SEP(mem_mgr gv; result_rep sh res pres; instance next_c penv).
+
+  Definition close_spec {rcd: Cursor.Rcd Otuple} (instance: iterator_invariant rcd) :=
+    WITH sh: share, gv: globals, penv: val, c: Cursor.cursor rcd
+  PRE [ _env OF (tptr tvoid) ]
+    PROP(Cursor.coherent c)
+    LOCAL(gvars gv; temp _env penv)
+    SEP(mem_mgr gv; instance c penv)
+  POST [ tvoid ]
+    PROP()
+    LOCAL()
+    SEP(mem_mgr gv). (* Something missing here. For now, the semantics of close are not well-defined. *)
   
-  Import btrees_sep btrees.
+  Definition iterator_methods {rcd: Cursor.Rcd Otuple}
+             (instance: iterator_invariant rcd) (pmtable: val) : mpred :=
+  EX sh: share, EX pinit: val, EX pnext: val, EX pclose: val,
+  !! readable_share sh && 
+  func_ptr' (init_spec instance) pinit *
+  func_ptr' (next_spec instance) pnext *
+  func_ptr' (close_spec instance) pclose *
+  data_at sh t_methods (pinit, (pnext, pclose)) pmtable.
 
-  Lemma node_dec_eq {X:Type} {h: EqDec X}: forall n1 n2: node X,
-      {n1 = n2} + {n1 <> n2}.
-  Proof.
-    fix hrec 1.
-    intros. decide equality. 
-    apply bool_dec. apply bool_dec. apply bool_dec.
-    decide equality. decide equality.
-    apply Int.eq_dec. apply Int.eq_dec.
-    apply Int.eq_dec. decide equality.
-  Qed.
-  
-  Lemma subchild_nth {X}: forall (n: node X) le, subchild n le -> exists i, nth_node_le i le = Some n.
-  Proof.
-    induction le.
-    easy.
-    intro h. inversion h. exists 0%nat. easy.
-    specialize (IHle H1). destruct IHle.
-    exists (S x)%nat.
-    easy.
-  Qed.
-  Open Scope nat_scope.
-  Lemma index_le_split_l': forall m n p, n <= m -> n <= index.max_nat m p.
-  Proof.
-    induction m; intros n p h. omega.
-    simpl. destruct p. assumption.
-    transitivity (S m). assumption.
-    apply le_n_S. apply IHm.
-    omega.
-  Qed.
+  Definition iterator_mpred {rcd: Cursor.Rcd Otuple} (c: Cursor.cursor rcd) (p: val) : mpred :=
+  EX instance: iterator_invariant rcd, EX pmtable: val, EX penv: val, 
+        data_at Ews t_iterator_t (pmtable, penv) p *
+        iterator_methods instance pmtable *
+        instance c penv.
 
-  Lemma index_le_r: forall n m, m <= index.max_nat n m.
-  Proof.
-    induction n.
-    simpl. easy.
-    destruct m.
-    omega.
-    simpl. apply le_n_S. apply IHn.
-  Qed.
-    
-  
-  Inductive subnode' {X : Type} : node X -> node X -> Prop :=
-    sub_refl' : forall n : node X, subnode' n n
-  | sub_ptr0' : forall (n m : node X) (le : listentry X) (First Last : bool) (x : X),
-               subnode' n m -> subnode' n (btnode X (Some m) le false First Last x)
-  | sub_child' : forall (n m : node X) (le : listentry X) (ptr0 : option (node X)) (First Last : bool) (x : X),
-      subnode' n m -> subchild m le -> subnode' n (btnode X ptr0 le false First Last x).
+  Print QEP.IndexJoin.
+  Definition indexjoin_invariant (attrs: list attribute): iterator_invariant (QEP.IndexJoin attrs outer_cursor inner_index) :=
+    fun 
 
-  Definition nodeDepthOrder X (n1 n2: node X) : Prop:= (node_depth n1 < node_depth n2)%nat.
-  
-  Lemma nodeDepthOrder_wf' {X} : forall depth, forall n, (node_depth n <= depth)%nat -> Acc (nodeDepthOrder X) n.
-  Proof.
-    unfold nodeDepthOrder.
-    induction depth; intros.
-    inversion H.
-    constructor. intros. omega.
-    constructor. intros.
-    inversion H.
-    + constructor. intros. apply IHdepth. omega.
-    + apply IHdepth. omega.
-  Defined.
-
-  Theorem nodeDepthOrder_wf (X: Type) : well_founded (nodeDepthOrder X).
-    red; intro; eapply nodeDepthOrder_wf'; eauto.
-  Defined.
-  
-  Program Definition sub_trans' {X: Type}: forall n m p: node X,
-      subnode' n m -> subnode' m p -> subnode' n p := fun n m =>
-    Fix (nodeDepthOrder_wf X) (fun p => subnode' n m -> subnode' m p -> subnode' n p) _.
-  Next Obligation.
-    inversion H1.
-    rewrite H3 in H0. assumption.
-    apply sub_ptr0'.
-    refine (H m0 _ _ _).
-    unfold nodeDepthOrder.
-    rewrite <- H4. simpl.
-    apply index.le_max_split_r. omega.
-    assumption.
-    assumption.
-    apply (sub_child' _ m0). apply H.
-    unfold nodeDepthOrder.
-    rewrite <- H5. apply subchild_nth in H3. destruct H3.
-    simpl.
-    apply (Nat.lt_le_trans _ (listentry_depth le)).
-    apply (nth_node_le_decrease _ le _ x1 H3).
-    apply index_le_split_l'. omega.
-    assumption.
-    assumption.
-    assumption.
- Defined.
-  
-  Lemma subnode_cons {X: Type} {heqdec: EqDec X} {n0} {ptr0} {k k'} {n n'} {le} {First Last} {x}
-        (h: subnode' n0 (btnode X (Some ptr0) (cons X (keychild X k' n') le) false First Last x)):
- n0 <> (btnode X (Some ptr0) (cons X (keychild X k' n') le) false First Last x) ->
- subnode' n0 (btnode X (Some ptr0) (cons X (keychild X k n) (cons X (keychild X k' n') le)) false First Last x).
-  Proof.
-    revert n0 h. fix hrec 1.
-    intros n0 hsubn0 hneq.
-    inversion hsubn0.
-    + easy.
-    + constructor. assumption.
-    + apply (sub_child' _ m). assumption.
-      apply sc_cons. assumption.
-  Qed.
-  
-  Lemma root_integrity_cons {X} {ptr0} {k k'} {n n'} {le} {First Last} {x}
-   (hint: root_integrity (btnode X (Some ptr0) (cons X (keychild X k n) (cons X (keychild X k' n') le)) false First Last x)):
-    root_integrity (btnode X (Some ptr0) (cons X (keychild X k' n') le) false First Last x).
-  Proof.
-    unfold root_integrity in hint |- *.
-    fix hrec 1.
-    intros n0 hn0.
-    inversion hn0.
-    ++ unfold node_integrity.
-       specialize (hint (btnode X (Some ptr0) (cons X (keychild X k n) (cons X (keychild X k' n') le)) false First Last x) (sub_refl _)).
-       inversion hint. assumption.
-    ++ apply hint.
-       constructor.
-    ++ apply hint.
-       apply sub_child.
-       apply sc_cons. assumption.
-    ++ apply hint.
-      admit. 
-Admitted.
-
-Definition btnode_induction {X} (P: node X -> Prop)
-           (hleaf: forall n, LeafNode n -> P n)
-           (hintern: forall (children: list (key * node X)) (h : children <> []) n First Last x,
-               Forall (P oo snd) children -> P n ->
-               P (btnode X (Some n)
-                         (fold_right (fun (kn : key * node X) le => let (k, n) := kn in cons X (keychild X k n) le) (nil X) children) false First Last x)) : forall n, root_integrity n -> P n.
-Proof.
-  fix hrec 1.
-  intros n rint. unfold root_integrity in rint.
-  destruct n as [[n0 |] le [] ].
-  + specialize (rint (btnode _ (Some n0) le true b b0 x) (sub_refl _)).
-    simpl in rint. easy.
-  + pose (children := listentry_rect X (fun _ => list (key * node X)) []
-                                     (fun e l acc => match e with
-                                                     | keychild k n' => (k, n') :: acc
-                                                     | _ => [] (* doesn't happen *) end) le).
-    simpl in children.
-    assert (le_not_nil: le <> nil X).
-    { intro. subst le. specialize (rint (btnode X (Some n0) (nil X) false b b0 x) (sub_refl _)).
-      easy. }
-    assert (children_not_nil: children <> []).
-    { destruct le. easy. simpl in children.
-      destruct e. specialize (rint (btnode X (Some n0) (cons X (keyval X k v x0) le) false b b0 x) (sub_refl _)). simpl in rint. inversion rint.
-      easy. }
-    replace le with (fold_right
-                       (fun (kn : key * node X) (le : listentry X) => let (k, n) := kn in cons X (keychild X k n) le)
-                       (nil X) children).
-  - apply (hintern children children_not_nil n0 b b0 x). clear le_not_nil children_not_nil.
-    rewrite Forall_forall. intros [childk childnode] hkn. simpl.
-    apply hrec. 
-    unfold root_integrity. intros subn hsubn.
-    apply rint.
-    apply sub_trans with (n1 := childnode). assumption.
-    apply sub_child.
-    apply In_nth with (d := (childk, childnode)) in hkn.
-    destruct hkn as [i [hi hnth]].
-    apply nth_subchild with (i := i).
-    subst children.
-    clear rint.
-    revert le hi hnth.
-    induction i ; destruct le.
-    ++ easy.
-    ++ destruct e. easy.
-       intros _ hnth. simpl in hnth. inversion hnth. easy.
-    ++ easy.
-    ++ simpl. destruct e. easy.
-       intros. simpl in *. apply IHi.
-       omega. easy.
-    ++ apply hrec. unfold root_integrity.
-       intros n hsn. apply rint.
-       apply sub_trans with (n2 := n0). assumption.
-       constructor.
-  - subst children. clear children_not_nil. destruct le.
-    easy. clear le_not_nil. simpl.
-    destruct e. specialize (rint _ (sub_refl _)). inversion rint.
-    revert k n rint.
-    induction le; simpl.
-    reflexivity.
-    intros k n rint.
-    destruct e. specialize (rint _ (sub_refl _)). inversion rint. inversion H0.
-    simpl in IHle. simpl. f_equal.
-    apply IHle.
-    intros n2 hn2.
-    inversion hn2.
-    ++ unfold node_integrity.
-       specialize (rint (btnode X (Some n0) (cons X (keychild X k n) (cons X (keychild X k0 n1) le)) false b b0 x) (sub_refl _)).
-       inversion rint. assumption.
-    ++ apply rint.
-       constructor.
-    ++ apply rint.
-       apply sub_child.
-       apply sc_cons. assumption.
-    ++ (* hn2 is obtained by transitivity. *)
-      
-      admit. 
-    + apply hleaf. easy.
-    + specialize (rint (btnode X None le false b b0 x) (sub_refl _)).
-      easy.
-Defined.
-
-    
-    intros n1 hn1.
-    inversion hn1.
-    simpl. specialize (rint (btnode X (Some n0) (cons X (keychild X k n) le) false b b0 x) (sub_refl _)) as rint1.
-    simpl in rint1. inversion rint1. 
-
-        
-      assert (hlenil : le <> nil X).
-      { intro hfalse. subst le. simpl in children. subst children. easy. }
-      
-      induction le.
-      ++ easy. 
-      ++ destruct e.
-         
-         pose proof (rint (btnode X (Some n0) (cons X (keyval X k0 v x0) le) false b b0 x) (sub_refl _)).
-         simpl in H0.
-         inversion H0.
-         Print sc_eq.
-         apply sc_eq.
-         simpl in hkn. destruct hkn.
-         
-         apply rint.
-      Print intern_le.
-      induction le. easy.
-      simpl in nint. inversion nint.
-      subst le. inversion H.
-      subst e. unfold In in hkn.
-      subst children. simpl in hkn.
-      
-
-
-  Lemma cursor_iter_next_abs_node {X} (r: relation X):
-    (get_numrec r > O)%nat ->
-    root_integrity (get_root r) ->
-    let c := moveToFirst (get_root r) [] 0 in
-    let l := abs_node (get_root r) in
-    forall n: nat,
-      getCKey (Nat.iter n (fun c' => RL_MoveToNext c' r) c) = option_map fst (nth_error l n).
-  Proof.
-    destruct r as [root proot]. case_eq root. intros o le isLeaf First Last x hroot. simpl.
-    intros hnempty rint.
-    assert (H : (exists n, o = Some n) \/ le <> nil X).
-    {
-      destruct o.
-      { left. exists n. reflexivity. }
-      { right. intro. subst le. unfold get_numrec in hnempty. simpl in hnempty. omega. }
-    }
-    induction n; simpl; intros; destruct isLeaf.
-    + assert (o = None /\ leaf_le le).
-      { unfold root_integrity, node_integrity in rint. specialize rint with root.
-        rewrite hroot in rint. apply rint. constructor. }
-      destruct H0. subst o. destruct H as [[] | ]. discriminate.
-      destruct le. contradiction.
-      simpl. inversion H1. subst e. simpl.
-      reflexivity.
-    + unfold root_integrity, node_integrity in rint. 
-      specialize (rint root). rewrite hroot in rint. specialize (rint (sub_refl _)).
-      destruct o; [ | easy].
-      inversion rint; subst le; clear H.
-    - simpl. Print moveToFirst.
-
-
-      
-      case_eq le; intro hle. simpl. rewrite hle in H.
-      unfold get_numrec, node_numrec in H. simpl in H. destruct o; try easy.
-      
-
-    
-  (* This predicate states that the btree and cursor physically represent
-     the abstract sequential scan iterator. *) (*
-  Definition seqscan_env_assert (bt: relation val) (c: cursor val)
-             (it: Cursor.cursor (SeqScan.SeqScan.build Otuple)) : mpred :=
-    (* The root node of the btree and its address. *)
-    let (root, pbt) := bt in
-    let l : list (tuple * val) :=
-        List.combine (Cursor.collection it) (List.map Vint (snd (List.split (abs_node relnode)))) in
-*)
-  Definition seqscan_iterator : iterator_class (SeqScan.SeqScan.build Otuple) :=
-    {|
-      env := btrees.relation val * btrees.cursor val;
-      env_assert := fun e it p =>
-                   let (rel, cur) := e in
-                   let (relnode, qrel) := rel in
-                   let l : list (tuple * val) :=
-                       List.combine (Cursor.collection it) (List.map Vint (snd (List.split (abs_node relnode)))) in
-                   EX qcur: val,
-                            !! (Forall (fun x: tuple * val => option_map Vint (getCRecord cur) = Some (snd x) ->
-                                                 fst (Cursor.next it) = Result (fst x)) l /\
-                            complete_cursor (snd e) (relnode, qrel) /\
-                                correct_depth (relnode, qrel) /\ root_wf (get_root (relnode, qrel)) /\
-                                root_wf relnode) &&
-                               iter_sepcon (fun x : tuple * val => let (t, p) := x in tuple_rep Tsh t p) l *
-                                        data_at Tsh t_seq_scan_env (qrel, qcur) p *
-                                        relation_rep (fst e) (btrees.get_numrec (fst e)) *
-                                        cursor_rep (snd e) (fst e) qcur;
-      env_init := fun e => (fst e, btrees.moveToFirst (fst (fst e)) (snd e) 0);
-      env_next := fun e => (fst e, btrees.moveToNext (snd e) (fst e));
-                             env_close := fun e => e; (* FreeRecord? *)
-       (* +axioms *)
-    |}.
-  
-  Definition seqscan_next_spec := (DECLARE _seq_scan_next (next_spec seqscan_iterator)).
 End Iterator.
 
-
-(* MATERIALIZE: WORK IN PROGRESS
-Definition materialize_spec :=
-  DECLARE _materialize
-    WITH sh: share, a: val, it: val, c: cursor
+Section Materialize.
+  Import db_operations FlatData Plans Signatures.
+  Import verif_queue2.
+  Import Cursor.
+  Existing Instance CompSpecs.
+  Definition abstract_cursor: Type  :=
+    {
+      rcd: Cursor.Rcd Otuple;
+      rep: iterator_class rcd;
+      concrete_env: rep.(env);
+      cursor: Cursor.cursor rcd
+    }.
+  Set Printing Universes.
+  Check val. Check abstract_cursor.
+  Definition materialize_spec :=
+    DECLARE _materialize
+    WITH gv: globals,
+             it: val, ac: abstract_cursor
     PRE [ _it OF (tptr t_iterator_t) ]
     PROP()
-    LOCAL(temp _it it; temp _a a)
-    SEP(iterator_rep sh c it)
-    POST [  *)
+    LOCAL(gvars gv; temp _it it)
+    SEP(mem_mgr gv; ac.(rep))
+    POST [ tptr t_fifo ]
+    EX r: val,
+    PROP()
+    LOCAL(temp ret_temp r)
+    SEP(mem_mgr gv; fifo [] r).
 
+  Definition materialize_spec :=
+    DECLARE _materialize
+    WITH gv: globals,
+             it: val, ac: abstract_cursor
+    PRE [ _it OF (tptr t_iterator_t) ]
+    PROP()
+    LOCAL(gvars gv; temp _it it)
+    SEP(mem_mgr gv; ac.(rep).(env_assert) ac.(concrete_env) ac.(cursor) it)
+    POST [ tptr t_fifo ]
+    EX r: val,
+    PROP()
+    LOCAL(temp ret_temp r)
+    SEP(mem_mgr gv; fifo (map snd (ac.(rcd).(collection))) r).
+
+  Let Gprog := ltac:(with_library prog [materialize_spec]).
+  
+End Iterator.
 
 Section Verif.
-  Import db_operations btrees_spec FiniteSet SortedAttributes.
-  Existing Instance db_operations_CompSpecs.
-  Let Gprog := ltac:(with_library prog [attribute_list_length_spec; RL_IsEmpty_spec; RL_CursorIsValid_spec]).
+  Import db_operations FiniteSet SortedAttributes.
+  Let Gprog := ltac:(with_library prog [attribute_list_length_spec]).
   Hint Resolve attribute_list_rep_local_facts : saturate_local.
   Hint Resolve attribute_lseg_rep_local_facts : saturate_local.
   Hint Resolve attribute_list_rep_valid_pointer : valid_pointer.
- (*
-  Lemma body_attribute_list_length: semax_body db_operations_Vprog Gprog f_attribute_list_length attribute_list_length_spec.
+ 
+  Lemma body_attribute_list_length: semax_body Vprog Gprog f_attribute_list_length attribute_list_length_spec.
   Proof.
     start_function.
     forward. forward.
@@ -528,15 +287,15 @@ Section Verif.
     - Exists l (@nil attribute) (Fset.elements _ attrs).
       entailer!. unfold attributes_rep, attribute_list_rep. simpl. entailer!.
     - entailer!.
-    - destruct l2. unfold attribute_list_rep, attribute_lseg_rep at 2. 
-      Intros. rewrite H0 in HRE. contradiction.
-      unfold attribute_list_rep; unfold attribute_lseg_rep at 2; fold attribute_lseg_rep. 
+    - destruct l2; unfold attribute_list_rep, attribute_lseg_rep at 2. 
+      Intros. subst x. contradiction.
+      fold attribute_lseg_rep. 
       Intros r sptr.
       forward.
       forward.
       Exists (r, l1 ++ [a], l2). entailer!.
-      split. rewrite semax_lemmas.cons_app in H. rewrite app_assoc in H. auto.
-      rewrite Zlength_app. rewrite Zlength_cons. simpl. reflexivity.
+      split. rewrite <- app_assoc. simpl. auto.
+      rewrite Zlength_app, Zlength_cons. reflexivity.
       unfold attribute_list_rep. cancel.
       revert l PNl. generalize l1. induction l0; intros. rewrite app_nil_l. simpl. Exists r sptr. entailer.
       simpl. Intros r0 sptr0. Exists r0 sptr0. entailer!.
@@ -546,7 +305,7 @@ Section Verif.
       rewrite Fset.cardinal_spec. rewrite Zlength_correct; auto. entailer!.
       unfold attributes_rep, attribute_list_rep. sep_apply attribute_lseg_nil. simpl. entailer!.
   Qed.
-  *)
+  
   Import btrees btrees_sep Signatures.Cursor.
   Lemma body_seqscan_next: semax_body db_operations_Vprog Gprog f_seq_scan_next seqscan_next_spec.
   Proof.
